proofs/OCamlFun.v
@@ -1,0 +1,3 @@
+Require Import RocqOfOCaml.Libraries.
+
+Definition id {a : Set} (value : a) : a := value.
