proofs/RocqOfOCaml.v
@@ -3,4 +3,25 @@ Require Export Basics.
 Require Export List.
 Require Export Tags.
 
+Require Lens.
+Require OCamlBigarray.
+Require OCamlChar.
+Require OCamlFormat.
+Require OCamlFun.
+Require OCamlHashtbl.
+Require OCamlIarray.
+Require OCamlInt.
+Require OCamlInt32.
+Require OCamlInt64.
+Require OCamlList.
+Require OCamlMap.
+Require OCamlOption.
+Require OCamlResult.
+Require OCamlSeq.
+Require OCamlSet.
+Require OCamlString.
+Require OCamlUchar.
+Require OCamlYojson.
+Require OCamlZ.
+
 Include Basics.
